Fix TLUL + new incr with spec

firmware/IncrementWait/CavaIncrementDevice.v
@@ -1,18 +1,25 @@
-From Coq Require Import
-     Lists.List
-     ZArith.ZArith.
+Require Import Coq.Lists.List.
+Require Import Coq.micromega.Lia.
+Require Import Coq.ZArith.ZArith.
+
+Require Import Cava.Expr.
+Require Import Cava.ExprProperties.
+Require Import Cava.Invariant.
+Require Import Cava.Primitives.
+Require Import Cava.Semantics.
+Require Import Cava.TLUL.
+Require Import Cava.Types.
+Require Import Cava.Util.BitArithmetic.
+Require Import Cava.Util.List.
+Require Import Cava.Util.Tactics.
+
+Require Import coqutil.Tactics.Simp.
+Require Import coqutil.Tactics.Tactics.
 
 Import ListNotations.
 
-From Cava Require Import
-     Expr
-     Primitives
-     Semantics
-     TLUL
-     Types
-     Util.BitArithmetic.
-
 Section Var.
+  Import Expr.
   Import ExprNotations.
   Import PrimitiveNotations.
 
@@ -25,6 +32,31 @@ Section Var.
   Definition Busy1      := Constant incr_state 1.
   Definition Busy2      := Constant incr_state 2.
   Definition Done       := Constant incr_state 3.
+
+  Definition inner
+    : Circuit _ [Bit; BitVec 32] (Bit ** BitVec 32)
+    := {{
+      fun valid data =>
+        let/delay '(istate; value) :=
+           let istate' :=
+               if istate == `Busy1` then `Busy2`
+               else if istate == `Busy2` then `Done`
+                    else if istate == `Done` then `Idle`
+                         else (* istate == `Idle` *)
+                           if valid then `Busy1`
+                           else `Idle` in
+
+           let value' :=
+               if istate == `Busy2` then value + `K 1`
+               else if istate == `Idle` then data
+                    else value in
+
+           (istate', value')
+             initially default
+           : denote_type (incr_state ** BitVec 32)
+        in
+        (istate == `Done`, value)
+       }}.
 
   Definition incr
     : Circuit _ [tl_h2d_t] tl_d2h_t
@@ -42,8 +74,8 @@ Section Var.
               , a_data
               , a_user
               ; d_ready) := tl_h2d in
-        (* Bit #2 of the address determines which register is being accessed
-           (STATUS or VALUE). Zero out the other bits. *)
+        (* Bit #2 of the address determines which register is being accessed *)
+        (*    (STATUS or VALUE). Zero out the other bits. *)
         let a_address := a_address & (`K 1` << 2) in
         let tl_h2d := (a_valid
                        , a_opcode
@@ -56,49 +88,45 @@ Section Var.
                        , a_user
                        , d_ready) in
 
-        let/delay '(istate, value; tl_d2h) :=
-           (* Compute the value of the status register *)
-           let status :=
-               if istate == `Done` then `K 4`
-               else if istate == `Busy1` || istate == `Busy2` then `K 2`
-                    else (* istate == `Idle` *) `K 1` in
+        let/delay '(busy, done, registers; tl_d2h) :=
+           let '(tl_d2h'; req) := `tlul_adapter_reg` tl_h2d registers in
+           let '(is_read, is_write, address, write_data; _write_mask) := req in
 
-           (* Handle the input:
-              - a_opcode = Get: the adapter will do all the work;
-              - a_opcode = PutFullData: further handling is needed, the adapter
-                will output more info to req. *)
-           let '(tl_d2h'; req) := `tlul_adapter_reg` tl_h2d (value :> status :> []) in
-           let '(is_read
-                 , is_write
-                 , address
-                 , write_data
-                 ; _write_mask) := req in
+           let '(inner_res_valid; inner_res) := `inner` (!busy && !done && is_write) write_data in
 
-           let istate' :=
-               if istate == `Busy1` then `Busy2`
-               else if istate == `Busy2` then `Done`
-                    else if istate == `Done` then
-                           if is_read && address == `K 0` then `Idle`
-                           else `Done`
-                         else (* istate == `Idle` *)
-                           if is_write then `Busy1`
-                           else `Idle` in
+           let busy' :=
+               if busy then !inner_res_valid
+               else !done && is_write in
 
-           let value' :=
-               if istate == `Busy2` then value + `K 1`
-               else if istate == `Idle` then write_data
-                    else value in
+           let done' :=
+               if busy then inner_res_valid
+               else if done then !(is_read && address == `K 0`)
+                    else done in
 
-           (istate', value', tl_d2h')
-             initially (0,
-                        (0,
-                         (false, (0, (0, (0, (0, (0, (0, (0, (false, false)))))))))))
-           : denote_type (incr_state ** BitVec 32 ** tl_d2h_t)
+           let registers' :=
+               if inner_res_valid then `replace` registers `K (sz:=1) 0` inner_res
+               else registers in
+
+           let registers' :=
+               if busy' then `replace` registers' `K (sz:=1) 1` `K 2`
+               else if done' then `replace` registers' `K (sz:=1) 1` `K 4`
+                    else `replace` registers' `K (sz:=1) 1` `K 1` in
+
+           (busy', done', registers', tl_d2h') initially default
+           : denote_type (Bit ** Bit ** Vec (BitVec 32) 2 ** tl_d2h_t)
         in
 
         tl_d2h
        }}.
 End Var.
+
+Definition sim {s i o} (c : Circuit s i o) (input : list (denote_type i))
+  : list (denote_type s * denote_type i * denote_type o) :=
+  fst (List.fold_left (fun '(acc, s) i =>
+                         let '(s', o) := step c s i in
+                         (acc ++ [(s, i, o)], s'))
+                      input
+                      ([], reset_state c)).
 
 Example sample_trace :=
   Eval compute in
@@ -117,20 +145,481 @@ Example sample_trace :=
         (set_a_data v
         (set_d_ready true tl_h2d_default))))) in
 
-    simulate incr
-             [ (nop, tt)
-               ; (read_reg 4, tt) (* status *)
-               ; (nop, tt)
-               ; (write_val 42, tt)
-               ; (nop, tt)
-               ; (nop, tt)
-               ; (read_reg 4, tt) (* status *)
-               ; (nop, tt)
-               ; (read_reg 0, tt) (* value *)
-               ; (nop, tt)
-               ; (read_reg 4, tt) (* status *)
-             ]%N.
+    sim incr
+        [ (nop, tt)
+          ; (read_reg 4, tt) (* status *)
+          ; (nop, tt)
+          ; (write_val 42, tt)
+          ; (nop, tt)
+          ; (nop, tt)
+          ; (read_reg 4, tt) (* status *)
+          ; (nop, tt)
+          ; (read_reg 0, tt) (* value *)
+          ; (nop, tt)
+          ; (read_reg 4, tt) (* status *)
+        ]%N.
 (* Print sample_trace. *)
+
+Section Spec.
+  Local Open Scope N.
+
+  Variant inner_state :=
+  | IISIdle
+  | IISBusy (data : N) (count : nat)
+  | IISDone (res : N).
+
+  Notation inner_repr := inner_state.
+
+  Global Instance inner_invariant : invariant_for inner inner_repr :=
+    fun (state : denote_type (state_of inner)) repr =>
+      let '(istate, value) := state in
+      match repr with
+      | IISIdle => istate = 0
+      | IISBusy data c => (0 < c <= 2)%nat /\ istate = N.of_nat c /\ value = data
+      | IISDone res => istate = 3 /\ value = res
+      end.
+
+  Definition inner_spec_step (input : denote_type (input_of inner)) repr :=
+    let '(valid, (data, tt)) := input in
+    match repr with
+    | IISIdle => if valid then IISBusy data 1 else IISIdle
+    | IISBusy data 2 => IISDone ((data + 1) mod 2^32)
+    | IISBusy data c => IISBusy data (c + 1)
+    | IISDone _ => IISIdle
+    end.
+
+  Instance inner_specification
+    : specification_for inner inner_repr :=
+    {| reset_repr := IISIdle;
+
+       update_repr :=
+         fun (input : denote_type (input_of inner)) repr =>
+           inner_spec_step input repr;
+
+       precondition :=
+         fun (input : denote_type (input_of inner)) repr => True;
+
+       postcondition :=
+         fun (input : denote_type (input_of inner)) repr
+           (output : denote_type (output_of inner)) =>
+           let repr' := inner_spec_step input repr in
+           match repr' with
+           | IISDone res => output = (true, res)
+           | _ => exists res, output = (false, res)
+           end;
+    |}.
+
+  Lemma inner_invariant_at_reset : invariant_at_reset inner.
+  Proof.
+    simplify_invariant inner. reflexivity.
+  Qed.
+
+  Lemma inner_invariant_preserved : invariant_preserved inner.
+  Proof.
+    intros (valid, (data, t)) state repr. destruct t.
+    cbn in * |-. destruct state as (istate, value).
+    intros repr' ? Hinvar Hprec; subst.
+    simplify_invariant inner.
+    simplify_spec inner.
+    cbv [inner inner_spec_step]. stepsimpl.
+    repeat (destruct_pair_let; cbn [fst snd]).
+    destruct repr as [|? iiscount|?]; logical_simplify; subst.
+    - destruct valid; cbn; try ssplit; lia.
+    - destruct iiscount as [|[|[|iiscount]]]; cbn; ssplit; lia.
+    - reflexivity.
+  Qed.
+
+  Lemma inner_output_correct : output_correct inner.
+  Proof.
+    intros (valid, (data, t)) state repr. destruct t.
+    cbn in * |-. destruct state as (istate, value).
+    remember (update_repr (c:=inner) (valid, (data, tt)) repr) as repr'.
+    intros Hinvar Hprec.
+    simplify_invariant inner.
+    simplify_spec inner.
+    cbv [inner inner_spec_step]. stepsimpl.
+    repeat (destruct_pair_let; cbn [fst snd]).
+    destruct repr as [|? iiscount|?]; logical_simplify; subst.
+    - destruct valid; eexists; cbn; try ssplit; reflexivity.
+    - destruct iiscount as [|[|[|iiscount]]]; try lia; try eexists; reflexivity.
+    - eexists. reflexivity.
+  Qed.
+
+  Existing Instances inner_invariant_at_reset inner_invariant_preserved
+           inner_output_correct.
+  Global Instance inner_correctness : correctness_for inner.
+  Proof. constructor; typeclasses eauto. Defined.
+
+
+  Variant repr_state :=
+  | RSIdle
+  | RSBusy (data : N)
+  | RSDone (res : N).
+
+  Notation repr := (repr_state * list N * list tl_h2d * inner_repr)%type.
+
+  Global Instance incr_invariant : invariant_for incr repr :=
+    fun (state : denote_type (state_of incr)) repr =>
+      let '((s_busy, (s_done, (s_regs, s_d2h))), (s_tlul, s_inner)) := state in
+      let '(r_state, r_regs, r_tlul, r_inner) := repr in
+      tlul_invariant (reg_count:=2) s_tlul r_tlul
+      /\ inner_invariant s_inner r_inner
+      /\ match r_state with
+        | RSIdle => s_busy = false /\ s_done = false
+                   /\ r_inner = IISIdle
+        | RSBusy data => s_busy = true /\ s_done = false
+                        /\ exists c, r_inner = IISBusy data c
+        | RSDone res => s_busy = false /\ s_done = true
+                       /\ (r_inner = IISDone res \/ r_inner = IISIdle)
+        end
+      /\ s_regs = r_regs.
+
+  Existing Instance tlul_specification.
+
+  Instance incr_specification
+    : specification_for incr repr :=
+    {| reset_repr := (RSIdle, [0; 0], [], IISIdle);
+
+       update_repr :=
+         fun (input : denote_type (input_of incr)) repr =>
+           let '(i_h2d, tt) := input in
+           let '(r_state, r_regs, r_tlul, r_inner) := repr in
+
+           let h2d := set_a_address (N.land (a_address i_h2d) 4) i_h2d in
+
+           let r_tlul' :=
+               let tlul_input := (h2d, (r_regs, tt)) in
+               update_repr (c:=tlul_adapter_reg (reg_count:=2))
+                           tlul_input r_tlul in
+
+           (* compute (some) tlul output *)
+           let '(is_read, is_write, address, write_data) :=
+               match outstanding_h2d (h2d :: r_tlul) with
+               | None => (false, false, 0, 0)
+               | Some h2d' =>
+                 if a_opcode h2d' =? Get then
+                   match outstanding_h2d r_tlul with
+                   | None => (a_valid h2d, false, a_address h2d, 0)
+                   | _ => (false, false, 0, 0)
+                   end
+                 else if a_opcode h2d' =? PutFullData then
+                   match outstanding_h2d r_tlul with
+                   | None => (false, a_valid h2d, a_address h2d, a_data h2d)
+                   | _ => (false, false, 0, 0)
+                   end
+                 else (false, false, 0, 0)
+               end in
+
+           let r_inner' :=
+               let inner_input := (match r_state with RSIdle => is_write | _ => false end, (write_data, tt)) in
+               update_repr (c:=inner) inner_input r_inner in
+
+           let r_state' :=
+               match r_state with
+               | RSDone _ =>
+                 if negb (is_read && (address =? 0)) then r_state
+                 else RSIdle
+               | _ =>
+                 match r_inner' with
+                 | IISBusy data _ => RSBusy data
+                 | IISDone res => RSDone res
+                 | _ => r_state
+                 end
+               end in
+
+           let r_regs' :=
+               match r_inner' with
+               | IISDone res => replace 0 res r_regs
+               | _ => r_regs
+               end in
+
+           let r_regs' :=
+               match r_state' with
+               | RSIdle => replace 1 1 r_regs'
+               | RSBusy _ => replace 1 2 r_regs'
+               | RSDone _ => replace 1 4 r_regs'
+               end in
+
+           (r_state', r_regs', h2d :: r_tlul, r_inner');
+
+       precondition :=
+         fun (input : denote_type (input_of incr)) repr =>
+           let '(i_h2d, tt) := input in
+           let '(r_state, r_regs, r_tlul, r_inner) := repr in
+
+           let h2d := set_a_address (N.land (a_address i_h2d) 4) i_h2d in
+
+           let tlul_input := (h2d, (r_regs, tt)) in
+
+           let prec_tlul :=
+               precondition (tlul_adapter_reg (reg_count:=2))
+                            tlul_input r_tlul in
+
+           let prec_inner :=
+               forall d2h is_read is_write address write_data write_mask,
+                 postcondition (tlul_adapter_reg (reg_count:=2))
+                               tlul_input r_tlul
+                               (d2h, (is_read, (is_write, (address, (write_data, write_mask)))))
+                 -> precondition inner (match r_state with RSIdle => is_write | _ => false end, (write_data, tt)) r_inner in
+
+           prec_tlul /\ prec_inner;
+
+       postcondition :=
+         fun (input : denote_type (input_of incr)) repr
+           (output : denote_type (output_of incr)) =>
+           let '(i_h2d, tt) := input in
+           let '(r_state, r_regs, r_tlul, r_inner) := repr in
+
+           let h2d := set_a_address (N.land (a_address i_h2d) 4) i_h2d in
+
+           let postc_tlul :=
+               let tlul_input := (h2d, (r_regs, tt)) in
+               exists req,
+                 postcondition (tlul_adapter_reg (reg_count:=2))
+                               tlul_input r_tlul
+                               (output, req) in
+           postc_tlul;
+    |}.
+
+  Lemma incr_invariant_at_reset : invariant_at_reset incr.
+  Proof.
+    simplify_invariant incr.
+    cbn. ssplit; try reflexivity.
+    apply (tlul_adapter_reg_invariant_at_reset (reg_count:=2)).
+  Qed.
+
+  Existing Instance tlul_adapter_reg_correctness.
+
+  (* TODO: move these lemmas to TLUL.v *)
+  Lemma outstanding_in_repr {reg_count : nat} : forall r_tlul t,
+      outstanding_h2d r_tlul = Some t ->
+      In t r_tlul.
+  Proof.
+    intros ? ?.
+    induction r_tlul; intros Houts; cbn in Houts.
+    - discriminate.
+    - destruct (outstanding_h2d r_tlul) eqn:Houts'.
+      + destruct d_ready.
+        * discriminate.
+        * apply in_cons. auto.
+      + destruct (a_valid a).
+        * inversion Houts. apply in_eq.
+        * discriminate.
+  Qed.
+
+  Lemma outstanding_a_valid {reg_count : nat} : forall r_tlul t,
+      outstanding_h2d r_tlul = Some t ->
+      a_valid t = true.
+  Proof.
+    intros ? ?.
+    induction r_tlul; intros Houts; cbn in Houts.
+    - discriminate.
+    - destruct (outstanding_h2d r_tlul) eqn:Houts'.
+      + destruct d_ready.
+        * discriminate.
+        * auto.
+      + destruct (a_valid a) eqn:Hvalid.
+        * inversion Houts. subst. assumption.
+        * discriminate.
+  Qed.
+
+  Lemma outstanding_prec {reg_count : nat} : forall tl_st r_tlul t,
+      tlul_invariant (reg_count:=reg_count) tl_st r_tlul ->
+      outstanding_h2d r_tlul = Some t ->
+      a_opcode t = Get \/ a_opcode t = PutFullData.
+  Proof.
+    intros ? ? ? Hinvar Houts. simpl in *.
+    apply (outstanding_in_repr (reg_count:=reg_count)) in Houts as Hin.
+    unfold tlul_invariant in Hinvar. logical_simplify.
+    eapply Forall_forall in H. 2: apply Hin.
+    apply H.
+    eapply (outstanding_a_valid (reg_count:=reg_count)).
+    apply Houts.
+  Qed.
+
+
+  Lemma incr_invariant_preserved : invariant_preserved incr.
+  Proof.
+    intros (h2d, t) state (((r_state, r_regs), r_tlul), r_inner). destruct t.
+    cbn in * |-. destruct state as ((busy, (done, (registers, d2h))), (tl_st, inner_st)).
+    destruct_tl_h2d. destruct_tl_d2h.
+    intros repr' ? Hinvar Hprec; subst.
+    simplify_invariant incr. logical_simplify. subst.
+    simplify_spec incr. logical_simplify. subst.
+    (* destruct Hprec as [regs Hprec]. *)
+    cbv [incr]. stepsimpl.
+    use_correctness.
+    match goal with
+    | H: (match outstanding_h2d (_::r_tlul) with | _ => _ end) |- _ =>
+      rename H into Htl_postc
+    end.
+    repeat (destruct_pair_let; cbn [fst snd]).
+    ssplit.
+    - eapply tlul_adapter_reg_invariant_preserved.
+      2: apply H.
+      + reflexivity.
+      + assumption.
+    - eapply inner_invariant_preserved.
+      2: apply H0.
+      + simpl in *.
+        destruct r_inner; try reflexivity.
+        destruct (outstanding_h2d r_tlul) eqn:Houts.
+        * destruct d_ready; logical_simplify; subst.
+          -- boolsimpl. destruct r_state; reflexivity.
+          -- eapply outstanding_prec in H as Hprec_t. 2: apply Houts.
+             destruct Hprec_t as [Hprec_t|Hprec_t];
+               rewrite Hprec_t in *; cbn in Htl_postc |- *; logical_simplify; subst;
+                 boolsimpl; destruct r_state; reflexivity.
+        * destruct a_valid eqn:Hvalid; logical_simplify; subst.
+          -- cbn in Htl_postc.
+             match goal with
+             | H: true = true -> _ |- _ =>
+               destruct H; try reflexivity; subst
+             end; cbn in Htl_postc; logical_simplify; subst;
+               boolsimpl; destruct r_state; logical_simplify; subst;
+                 reflexivity.
+          -- boolsimpl; destruct r_state; reflexivity.
+      + match goal with
+        | H: context [_ -> precondition inner _ r_inner] |- _ =>
+          eapply H
+        end.
+        do 8 eexists. ssplit.
+        1-2: reflexivity.
+        apply Htl_postc.
+    - match goal with
+      | H: context [_ -> precondition inner _ r_inner] |- _ => clear H
+      end.
+      destruct r_inner; destruct r_state; destruct inner_st;
+        unfold inner_invariant in H0; logical_simplify; subst;
+          try discriminate;
+          try (destruct H4; discriminate).
+      all: destruct (outstanding_h2d r_tlul) eqn:Houts;
+        cbn [outstanding_h2d] in Htl_postc |- *; rewrite Houts in Htl_postc |- *.
+      all: tlsimpl; destruct d_ready; logical_simplify; subst; boolsimpl.
+      all: cbn; try (ssplit; reflexivity).
+      all: try (eapply outstanding_prec in H;
+                try match goal with
+                    | H: outstanding_h2d _ = Some _ |- outstanding_h2d _ = Some _ =>
+                      apply H
+                    end; destruct H; rewrite H in Htl_postc |- *; cbn in Htl_postc |- *;
+                logical_simplify; subst; ssplit;
+                try (left; reflexivity);
+                try (right; reflexivity);
+                reflexivity).
+      all: try (destruct a_valid; simplify_spec (tlul_adapter_reg (reg_count:=2));
+                tlsimpl; destruct H2;
+                try match goal with
+                    | H: true = true -> _ |- _ =>
+                      destruct H; try reflexivity; subst
+                    end; cbn in Htl_postc; logical_simplify; subst; cbn; ssplit;
+                  try eexists; reflexivity).
+      all: try (destruct a_valid; ssplit;
+                try (left; reflexivity);
+                try (right; reflexivity);
+                reflexivity).
+      all: try (destruct a_valid; simplify_spec (tlul_adapter_reg (reg_count:=2));
+                tlsimpl; destruct H2;
+                try match goal with
+                    | H: true = true -> _ |- _ =>
+                      destruct H; try reflexivity; subst
+                    end; cbn in Htl_postc; logical_simplify; subst;
+                boolsimpl; destruct (negb (N.land a_address 4 =? 0)) eqn:Haddr;
+                cbn; try (rewrite Haddr); ssplit;
+                try (left; reflexivity);
+                try (right; reflexivity);
+                reflexivity).
+      all: (inversion H4; subst; clear H4;
+            destruct x as [|[|[|?]]]; cbn; ssplit;
+            try eexists;
+            try (left; reflexivity);
+            try (right; reflexivity);
+            try reflexivity;
+            exfalso; lia).
+    - match goal with
+      | H: context [_ -> precondition inner _ r_inner] |- _ => clear H
+      end.
+      destruct r_inner; destruct r_state; destruct inner_st;
+        unfold inner_invariant in H0; logical_simplify; subst;
+          try discriminate.
+      all: destruct (outstanding_h2d r_tlul) eqn:Houts;
+        cbn [outstanding_h2d] in Htl_postc |- *; rewrite Houts in Htl_postc |- *.
+      all: tlsimpl; destruct d_ready; logical_simplify; subst; boolsimpl.
+      all: try reflexivity.
+      all: try (eapply outstanding_prec in H;
+                try match goal with
+                    | H: outstanding_h2d _ = Some _ |- outstanding_h2d _ = Some _ =>
+                      apply H
+                    end; destruct H; rewrite H in Htl_postc |- *; cbn in Htl_postc |- *;
+                logical_simplify; subst; cbn; reflexivity).
+      all: try (destruct a_valid; simplify_spec (tlul_adapter_reg (reg_count:=2));
+                tlsimpl; destruct H2;
+                try match goal with
+                    | H: true = true -> _ |- _ =>
+                      destruct H; try reflexivity; subst
+                    end; cbn in Htl_postc; logical_simplify; subst; reflexivity).
+      all: try (destruct a_valid; simplify_spec (tlul_adapter_reg (reg_count:=2));
+                tlsimpl; destruct H2;
+                try match goal with
+                    | H: true = true -> _ |- _ =>
+                      destruct H; try reflexivity; subst
+                    end; cbn in Htl_postc; logical_simplify; subst;
+                boolsimpl; destruct (negb (N.land a_address 4 =? 0)) eqn:Haddr;
+                cbn; try (rewrite Haddr); reflexivity).
+      all: try (inversion H4; subst; clear H4;
+            destruct x as [|[|[|?]]]; try reflexivity; exfalso; lia).
+      all: try (destruct H4; discriminate).
+  Qed.
+
+  Lemma incr_output_correct : output_correct incr.
+  Proof.
+    intros (h2d, t) state (((r_state, r_regs), r_tlul), r_inner). destruct t.
+    cbn in * |-. destruct state as ((busy, (done, (registers, d2h))), (tl_st, inner_st)).
+    destruct_tl_h2d. destruct_tl_d2h.
+    intros Hinvar Hprec; subst.
+    simplify_invariant incr. logical_simplify. subst.
+    simplify_spec incr. logical_simplify. subst.
+    cbv [incr]. stepsimpl.
+    use_correctness.
+    match goal with
+    | H: (match outstanding_h2d (_::r_tlul) with | _ => _ end) |- _ =>
+      rename H into Htl_postc
+    end.
+    repeat (destruct_pair_let; cbn [fst snd]).
+    tlsimpl.
+    destruct r_inner; destruct r_state; destruct inner_st;
+      unfold inner_invariant in H0; logical_simplify; subst;
+        try discriminate;
+        try (destruct H5; discriminate).
+    all: destruct (outstanding_h2d r_tlul) eqn:Houts;
+      cbn [outstanding_h2d] in Htl_postc |- *; rewrite Houts in Htl_postc |- *.
+    all: tlsimpl; destruct d_ready; logical_simplify; subst; boolsimpl.
+    all: do 9 eexists.
+    all: ssplit; try reflexivity; tlsimpl; ssplit; try reflexivity; try assumption.
+    all: try (eapply outstanding_prec in H;
+              try match goal with
+                  | H: outstanding_h2d _ = Some _ |- outstanding_h2d _ = Some _ =>
+                    apply H
+                  end; destruct H; rewrite H in Htl_postc |- *; cbn in Htl_postc |- *;
+              logical_simplify; subst; ssplit;
+              try (left; reflexivity);
+              try (right; reflexivity);
+              try assumption;
+              reflexivity).
+    all: try (destruct a_valid; simplify_spec (tlul_adapter_reg (reg_count:=2));
+              tlsimpl; destruct H2;
+              try match goal with
+                  | H: true = true -> _ |- _ =>
+                    destruct H; try reflexivity; subst
+                  end; cbn in Htl_postc; logical_simplify; subst; cbn; ssplit;
+              try eexists; try assumption; reflexivity).
+    Unshelve. all: auto.
+  Qed.
+
+  Existing Instances incr_invariant_at_reset incr_invariant_preserved
+           incr_output_correct.
+  Global Instance incr_correctness : correctness_for incr.
+  Proof. constructor; typeclasses eauto. Defined.
+End Spec.
 
 Require Import Coq.micromega.Lia.
 
